---
title: Green
date: 2022-12-29
author: bosonicli
tags:
-   Ether
---

[toc]

# Green

about complex analyticity, Green's function, linear response and so on

## Kramas-Kronig relations

by definition of contour integration, 

$$
\begin{aligned}
    0 &= \oint \frac{ \chi( \omega ' )}{ \omega ' - \omega } d \omega ' \\
    &= \mathcal{P} \int_{-\infty}^{\infty} \frac{ \chi( \omega ' )}{ \omega ' - \omega } d \omega ' - i \pi \chi(\omega)    \\
    \chi(\omega) &= \frac{1}{ i \pi } \mathcal{P} \int_{-\infty}^{\infty} \frac{ \chi( \omega ' )}{ \omega ' - \omega } d \omega '
\end{aligned}
$$

on real axis, 

$$
\begin{aligned}
    & \lim_{\epsilon \to 0^{+}} \int_{a}^{b} \frac{f(x)}{x \pm i\epsilon} dx  \\
    &= \mp i \pi f(0) + \mathcal{P} \int_{a}^{b} \frac{f(x)}{x} dx
\end{aligned}
$$

by taking \\( f(x) \equiv 1 \\) we have, 

$$
\begin{aligned}
    & \lim_{\epsilon \to 0^{+}} \frac{1}{x \pm i\epsilon}   \\
    &= \mp i \pi \delta(0) + \mathcal{P} ( \frac{1}{x} )
\end{aligned}
$$

by taking \\( \int_{0}^{\infty} dt f(E) exp( +iEt ) \\) to \\( \int_{0}^{\infty} dt f(E) exp( +iEt-\epsilon t ) = \frac{f(E)}{ E + i \epsilon } \\), we have deduced the Heitler function

$$
\begin{aligned}
    & \int_{-\infty}^{\infty} e^{ +i \omega \tau } \Theta(\tau) d \tau  \\
    &= \int_{0}^{\infty} e^{ +i \omega \tau } d \tau    \\
    &= \frac{i}{ \omega + i 0^{+} } \\
    &= \pi \delta(\omega) + i \mathcal{P} ( \frac{1}{\omega} )
\end{aligned}
$$

## Response

$$
\begin{aligned}
    f(\omega) &\equiv \frac{G(\omega)}{ - i ( \omega + i 0^{+} ) }    \\
    &= \frac{ G'(\omega) + i G'' (\omega) }{ - i ( \omega + i 0^{+} ) }    \\
    f'(\omega) &=
    \begin{cases}
        - \frac{ G'' (\omega) }{\omega} & (\omega \neq 0) \\
        \delta(\omega=0) \pi G'(0) & (\omega = 0)
    \end{cases} \\
    f''(\omega) &=
    \begin{cases}
        \frac{ G' (\omega) }{\omega} & (\omega \neq 0) \\
        \delta(\omega=0) \pi G''(0) & (\omega = 0)
    \end{cases}
\end{aligned}
$$

## Equation of Motion

$$
\begin{aligned}
    ( \omega - \hat{H} ) G(\omega) &= 1 \\
    G(\omega) & \equiv ( \omega - \hat{H} )^{-1}
\end{aligned}
$$

## Analytic Continuation

$$
\begin{aligned}
    G^{R}(\omega) & \equiv G ( \omega + i 0^{+} )   \\
    G^{A}(\omega) & \equiv G ( \omega - i 0^{+} )
\end{aligned}
$$

$$
\begin{aligned}
    G( i \omega_{n} ) & = \int_{0}^{\beta} e^{ i \omega_{n} \tau } G(\tau) d \tau   \\
    G(\tau) & = \frac{1}{\beta} \Sigma_{ i \omega_{n} } e^{ - i \omega_{n} \tau } G( i \omega_{n} \tau )
\end{aligned}
$$

$$
\begin{aligned}
    G(z) & \equiv \mathcal{P} \int \left[ \frac{1}{z-\omega} ( - \frac{ImG(\omega)}{\pi}) \right] d \omega  \\
    & + i \mathcal{P} \int \left[ \frac{1}{z-\omega} \frac{ReG(\omega)}{\pi} \right] d \omega   \\
    G( i \omega_{n} ) & = \int \left[ \frac{1}{ i \omega_{n}- \omega } ( - \frac{ImG^{R}(\omega)}{\pi}) \right] d \omega    \\& = \int \left[ \frac{ A(\omega) }{ i \omega_{n}- \omega } \right] d \omega
\end{aligned}
$$

$$
\begin{aligned}
    G( i \omega_{n}) & = \int A(\omega) \frac{1}{ i \omega_{n} - \omega } d \omega  \\
    & \Updownarrow  \\
    G( \tau) & = \int A(\omega) \frac{ e ^{ - \tau \omega } }{ 1 + e^{ - \tau \beta } } d \omega    \\
    K( i \omega_{n} , \omega ) & \equiv \frac{1}{ i \omega_{n} - \omega }   \\
    & \Updownarrow  \\
    K( \tau, \omega ) & = \frac{ e ^{ - \tau \omega } }{ 1 + e^{ - \tau \beta } }
\end{aligned}
$$
