---
title: 2023-02-18 - Symmetry
date: 2023-02-18
author: bosonicli
tags:
-   Ether
---

[toc]

# Active / Passive Transformation

$$
\begin{aligned}
    \delta &= \delta_{0} + \delta x^{\mu} \partial_{\mu}
\end{aligned}
$$

Take Spacetime Translation as example

$$
\begin{aligned}
    x^{\mu} & \rightarrow x^{\mu} + a^{\mu} \\
    \delta \phi &= 0    \\
    \phi'(x) &= \phi(x-a)   \\
    &= \phi(x) - a^{\mu} \partial_{\mu} \phi    \\
    \delta_{0} \phi &= \delta \phi - a^{\mu} \partial_{\mu} \phi \\
    &= a^{\mu} \partial_{\mu} \phi
\end{aligned}
$$

# Lagrangian

$$
\begin{aligned}
    S & \equiv \int dx \mathcal{L} \left[ x , \phi, \partial \phi \right]   \\
    \delta S &= \int ( \delta(dx) \mathcal{L} + dx \delta(\mathcal{L}) )    \\
    \delta (dx) &= dx ( \partial_{\mu} \delta x^{\mu} )    \\
    \delta \mathcal{L} &= \delta_{0} \mathcal{L} + \delta x^{\mu} \partial_{\mu} \mathcal{L}    \\
    &= \delta x^{\mu} \partial_{\mu} \mathcal{L} + \delta_{0} \phi \frac{ \partial \mathcal{L} }{ \partial \phi} + \delta_{0} \partial_{\mu} \phi \frac{ \partial \mathcal{L} }{ \partial ( \partial_{\mu} \phi )} \\
    &= \delta x^{\mu} \partial_{\mu} \mathcal{L} + \partial_{\mu} ( \frac{ \partial \mathcal{L} }{ \partial ( \partial_{\mu} \phi )} \delta_{0} \phi ) + \delta_{0} \phi (\frac{ \partial \mathcal{L} }{ \partial \phi } - \partial_{\mu} \frac{ \partial \mathcal{L} }{ \partial ( \partial_{\mu} \phi ) })    \\
    \delta S &= \int \left[ \partial_{\mu} ( \delta x^{\mu} \mathcal{L} +\frac{ \partial \mathcal{L} }{ \partial ( \partial_{\mu} \phi )} \delta_{0} \phi ) + \delta_{0} \phi (\frac{ \partial \mathcal{L} }{ \partial \phi } - \partial_{\mu} \frac{ \partial \mathcal{L} }{ \partial ( \partial_{\mu} \phi ) }) \right] \\
    &= \int \left[ \partial_{\mu} j^{\mu} + \delta_{0} \phi (\frac{ \partial \mathcal{L} }{ \partial \phi } - \partial_{\mu} \frac{ \partial \mathcal{L} }{ \partial ( \partial_{\mu} \phi ) }) \right] \\
    0 &= \partial_{\mu} j^{\mu} \\
    0 &= \frac{ \partial \mathcal{L} }{ \partial \phi } - \partial_{\mu} \frac{ \partial \mathcal{L} }{ \partial ( \partial_{\mu} \phi ) }
\end{aligned}
$$

Noether's Theorem

$$
\begin{aligned}
    j^{\mu} & \equiv \delta x^{\mu} \mathcal{L} + \frac{ \partial \mathcal{L} }{ \partial ( \partial_{\mu} \phi )} \delta_{0} \phi \\
    &= \delta x^{\mu} \mathcal{L} + \frac{ \partial \mathcal{L} }{ \partial (\partial_{\mu} \phi) } ( - \delta x^{\nu} \partial_{\nu} \phi ) + \frac{ \partial \mathcal{L} }{ \partial ( \partial_{\mu} \phi )} \delta \phi    \\
    &= ( \mathcal{L} g_{\nu}^{\mu} - \frac{ \partial \mathcal{L} }{ \partial ( \partial_{\mu} \phi ) } \partial_{\nu} \phi ) \delta x^{\nu} + \frac{ \partial \mathcal{L} }{ \partial ( \partial_{\mu} \phi )} \delta \phi
\end{aligned}
$$

# Spacetime Translational Symmetry

$$
\begin{aligned}
    \begin{cases}
        \delta x^{\mu} &= a^{\mu}   \\
        \delta \phi &= 0
    \end{cases}
\end{aligned}
$$

So

$$
\begin{aligned}
    j^{\mu} &= ( \mathcal{L} g_{\nu}^{\mu} - \frac{ \partial \mathcal{L} }{ \partial ( \partial_{\mu} \phi ) } \partial_{\nu} \phi ) a^{\nu} \\
    &= ( - \mathcal{L} g^{ \mu \nu } + \frac{ \partial \mathcal{L} }{ \partial ( \partial_{\mu} \phi ) } \partial^{\nu} \phi ) a_{\nu}  \\
    & \equiv T^{ \mu \nu } a_{\nu}  \\
    \partial_{\mu} T^{ \mu \nu } &= 0
\end{aligned}
$$

Where \\( T^{ \mu \nu } \\) is the E-M Tensor

# Massless Free Boson

$$
\begin{aligned}
    \mathcal{L} & \equiv \frac{1}{2} ( \partial_{\mu} \phi )^2  \\
    &
    \begin{cases}
        \delta \phi &= \alpha   \\
        \delta x^{\mu} &= 0
    \end{cases} \\
    j^{\mu} &= \alpha \partial^{\mu} \phi   \\
    0 &= \partial_{\mu} ( \partial^{\mu} \phi ) \\
    &= \square \phi
\end{aligned}
$$

# Non-Abelian Gauge Field

Under Global Unitary Transformation

$$
\begin{aligned}
    \phi(x) & \rightarrow U \phi(x)   \\
    \mathcal{L} &= \partial \phi^{\dagger} \partial \phi - V( \phi^{\dagger} \phi )
\end{aligned}
$$

Under Local Unitary Transformation

$$
\begin{aligned}
    \phi(x) & \rightarrow U(x) \phi(x)   \\
    \mathcal{L} &= D \phi^{\dagger} D \phi - V( \phi^{\dagger} \phi )   \\
    D_{\mu} & \equiv \partial_{\mu} - i A_{\mu} \\
    A_{\mu} & \rightarrow U A_{\mu} U^{\dagger} + i U \partial_{\mu} U^{\dagger}
\end{aligned}
$$

For example the \\( SU(N) \\) generators \\( T^{a} \\)

$$
\begin{aligned}
    U & \equiv e^{ i \theta T } \\
    A_{\mu} & \rightarrow A_{\mu} + i \theta^{a} \left[ T^{a} , A_{\mu} \right] + \partial_{\mu} \theta^{a} T^{a}
\end{aligned}
$$

# Problems remain

+   Current and Local Transformation
