---
title: 2023-02-24 - Dirac
date: 2023-02-24
author: bosonicli
tags:
-   Ether
---

[toc]

# Dirac Spinor

Covariant Derivative

$$
\begin{aligned}
    \partial_{\mu} & \equiv ( \frac{1}{c} \frac{\partial}{ \partial t } , \frac{\partial}{ \partial x } , \frac{\partial}{ \partial y } , \frac{\partial}{ \partial z } )
\end{aligned}
$$

Dirac Equation

$$
\begin{aligned}
    0 &= ( i \gamma^{\mu} \partial_{\mu} - m ) \psi \\
    \left\{ \gamma^{\mu} , \gamma^{\nu} \right\} &= 2 g^{ \mu \nu } \\
    \gamma^{0} &=
    \begin{pmatrix}
        \mathbf{I} \quad \mathbf{0} \\
        \mathbf{0} \quad \mathbf{-I}
    \end{pmatrix}   \\
    \gamma^{i} &=
    \begin{pmatrix}
        \mathbf{0} \quad \sigma^{i} \\
        -\sigma^{i} \quad \mathbf{0}
    \end{pmatrix}   \\
    \gamma^{5} & \equiv i \gamma^{0} \gamma^{1} \gamma^{2} \gamma^{3}   \\
    &=
    \begin{pmatrix}
        \mathbf{0} \quad \mathbf{I} \\
        \mathbf{I} \quad \mathbf{0}
    \end{pmatrix}   \\
    ( \gamma^{5} )^2 &= 1   \\
    \left\{ \gamma^{5} , \gamma^{\mu} \right\} &= 0 \\
    \gamma^{5} \gamma^{0} \gamma^{i} &=
    \begin{pmatrix}
        \sigma^{i} \quad \mathbf{0} \\
        \mathbf{0} \quad \sigma^{i}
    \end{pmatrix}   \\
    &= \sigma^{i} \otimes \mathbf{I_{2}}
\end{aligned}
$$

Spinor

$$
\begin{aligned}
    \psi (x^{\mu}) & \equiv u(p^{\mu}) e^{ - i p x }    \\
    0 &= ( \gamma^{\mu} \partial_{\mu} - m ) u(p^{\mu})   \\
    ( \vec{\sigma} \cdot \vec{p} )^2 &= \lvert \vec{p} \rvert ^2    \\
    &= E^2 -m^2 \\
    u^{1} (p^{\mu}) &=
    \begin{pmatrix}
        \begin{pmatrix}
            1   \\
            0
        \end{pmatrix}   \\
        \frac{ \vec{\sigma} \cdot \vec{p} }{ E + m }
        \begin{pmatrix}
            1   \\
            0
        \end{pmatrix}
    \end{pmatrix}   \\
    u^{2} (p^{\mu}) &=
    \begin{pmatrix}
        \begin{pmatrix}
            0   \\
            1
        \end{pmatrix}   \\
        \frac{ \vec{\sigma} \cdot \vec{p} }{ E + m }
        \begin{pmatrix}
            0   \\
            1
        \end{pmatrix}
    \end{pmatrix} \\
    u^{3} (p^{\mu}) &=
    \begin{pmatrix}
        \frac{ \vec{\sigma} \cdot (\vec{-p}) }{ - E + m }
        \begin{pmatrix}
            1   \\
            0
        \end{pmatrix}   \\
        \begin{pmatrix}
            1   \\
            0
        \end{pmatrix}
    \end{pmatrix}   \\
    u^{4} (p^{\mu}) &=
    \begin{pmatrix}
        \frac{ \vec{\sigma} \cdot (\vec{-p}) }{ - E + m }
        \begin{pmatrix}
            0   \\
            1
        \end{pmatrix}   \\
        \begin{pmatrix}
            0   \\
            1
        \end{pmatrix}
    \end{pmatrix}   \\
    E u^{1,2} (p^\mu) &= \sqrt{ \vec{p}^2 + m^2 } u^{1,2} (p^{\mu})   \\
    E u^{3,4} (p^\mu) &= - \sqrt{ \vec{p}^2 + m^2 } u^{3,4} (p^{\mu})
\end{aligned}
$$

## Conjugation / Helicity / Chirality

Charge Conjugation \\( \mathcal{C} \\)

$$
\begin{aligned}
    v^{2} (p^{\mu}) & \equiv u^{3} (-p^{\mu}) \\
    &=
    \begin{pmatrix}
        \frac{ \vec{\sigma} \cdot \vec{p} }{ E + m }
        \begin{pmatrix}
            1   \\
            0
        \end{pmatrix}   \\
        \begin{pmatrix}
            1   \\
            0
        \end{pmatrix}
    \end{pmatrix}   \\
    E v^{2,1} (p^\mu) &= \sqrt{ \vec{p}^2 + m^2 } v^{2,1} (p^{\mu})   \\
    \psi^{3} &= u^{3} (p^{\mu}) e^{ - i p x }   \\
    &= v^{2} (-p^{\mu}) e^{ i (-p) x }    \\
    \psi^{4} &= v^{1} (-p^{\mu}) e^{ i (-p) x }    \\
    0 &= ( \gamma^{\mu} \partial_{\mu} + m ) v(p^{\mu})
\end{aligned}
$$

Hamiltonian

$$
\begin{aligned}
    \hat{H} & \equiv p^{0} \\
    &= \gamma^{0} ( \gamma^{0} p^{0} )   \\
    &= \gamma^{0} m - \gamma^{0} \gamma^{i} p^{i}   \\
    &= ( m + \gamma^{i} p^{i} ) \gamma^{0}
\end{aligned}
$$

Helicity

$$
\begin{aligned}
    \hat{h} & \equiv \frac{ \vec{\sigma} \cdot \vec{p} }{\lvert\vec{p}\rvert} \\
    &= \frac{p^{i}}{\lvert\vec{p}\rvert} \gamma^{5} \gamma^{0} \gamma^{i} \\
    \left[ \hat{H} , \hat{h} \right] &=0    \\
    \hat{h}^2 &= \mathbf{I_{2}}  \\
    h &= \pm 1
\end{aligned}
$$

$$
\begin{aligned}
    \hat{h} u^{1} ( p^{\mu}, m ) &=
    \frac{E-m}{\lvert\vec{p}\rvert}
    \begin{pmatrix}
        \frac{ \vec{\sigma} \cdot \vec{p} }{ E - m }
        \begin{pmatrix}
            1   \\
            0
        \end{pmatrix}   \\
        \begin{pmatrix}
            1   \\
            0
        \end{pmatrix}
    \end{pmatrix}   \\
    &= \frac{E-m}{\lvert\vec{p}\rvert} v^{2} ( p^{\mu} , - m )  \\
    &=
    \begin{cases}
        u^{1} ( p^{\mu}, m ) \quad ( \vec{\sigma} \parallel \vec{p} )   \\
        - u^{1} ( p^{\mu}, m ) \quad ( \vec{\sigma} \parallel \vec{-p} )
    \end{cases}
\end{aligned}
$$
