---
title: 2023-03-15 - Tensor
date: 2023-03-15
author: bosonicli
tags:
-   Ether
---

[toc]

# Jacobian

$$
\begin{aligned}
    J_{\alpha}^{\beta} & \equiv \frac{ \partial y_{\alpha} }{ \partial x_{\beta} }  \\
    \vec{e_{i}} & \equiv \frac{ \partial \vec{r} }{ \partial x^{i} }    \\
    \hat{e_{i}} & \equiv \frac{\vec{e_{i}}}{\lvert e_{i} \rvert}    \\
    \vec{e_{x}^{\beta}} &= \frac{ \partial \vec{r} }{ \partial x^{\beta} }    \\
    &= \frac{ \partial \vec{r} }{ \partial y_{\alpha} } \frac{ \partial y_{\alpha} }{ \partial x_{\beta} }  \\
    &= J_{\alpha}^{\beta} \vec{e_{y}^{\alpha}} \\
    ( \vec{e_{x}} )^{T} &= J^{T} ( \vec{e_{y}} )^{T}  \\
    v & \to J v \\
    u^{T} v & \to ( J u )^{T} ( J v )   \\
    &= u^{T} J^{T} J v  \\
    &= u^{T} G v \\
    G & \equiv J^{T} J  \\
    \lvert det(G) \rvert &= \lvert det(J) \rvert^2  \\
    \hat{e_{x}^{\beta}} &= \frac{\vec{e_{x}^{\beta}}}{\lvert e_{i}^{\beta} \rvert}  \\
    &= \frac{ J_{\alpha}^{\beta} \vec{e_{y}^{\alpha}} }{ G_{\beta}^{\beta} }    \\
    ( \hat{e_{x}} )^{T} &=  diag( J^{T} J )^{-\frac{1}{2}} J^{T} ( \hat{e_{y}} )^{T}
\end{aligned}
$$

Polar Coordinate

$$
\begin{aligned}
    ( x , y ) & \to ( r , \theta )  \\
    &
    \begin{cases}
        x &= r cos \theta \\
        y &= r sin \theta
    \end{cases} \\
    J &= \frac{ \partial ( x , y ) }{ \partial ( r , \theta ) }  \\
    &=
    \begin{pmatrix}
        \frac{ \partial x }{ \partial r } \quad & \frac{ \partial x }{ \partial \theta }  \\
        \frac{ \partial y }{ \partial r } \quad & \frac{ \partial y }{ \partial \theta }
    \end{pmatrix}   \\
    &=
    \begin{pmatrix}
        cos \theta \quad & - r sin \theta  \\
        sin \theta \quad & r cos \theta
    \end{pmatrix}   \\
    \lvert det(J) \rvert &= r   \\
    J^{-1} &= \frac{1}{r}
    \begin{pmatrix}
        r cos \theta \quad & r sin \theta   \\
        - sin \theta \quad & cos \theta
    \end{pmatrix}   \\
    ( \hat{r} , \hat{\theta} )^{T} &= diag( J^{T} J )^{-\frac{1}{2}} J^{T} ( \hat{x} , \hat{y} )^{T}    \\
    &=
    \begin{pmatrix}
        cos \theta \quad & sin \theta   \\
        - sin \theta \quad & cos \theta
    \end{pmatrix}
    ( \hat{x} , \hat{y} )^{T}
\end{aligned}
$$

Spherical Coordinate

$$
\begin{aligned}
    ( x , y , z ) & \to ( \rho , \theta , \phi )  \\
    &
    \begin{cases}
        x &= \rho sin \theta cos \phi \\
        y &= \rho sin \theta sin \phi   \\
        z &= \rho cos \theta
    \end{cases} \\
    J &= \frac{ \partial ( x , y , z ) }{ \partial ( r , \theta , \phi ) }  \\
    &=
    \begin{pmatrix}
        \frac{ \partial x }{ \partial \rho } \quad \frac{ \partial x }{ \partial \phi } \quad & \frac{ \partial x }{ \partial \phi }  \\
        \frac{ \partial z }{ \partial \rho } \quad \frac{ \partial z }{ \partial \phi } \quad & \frac{ \partial z }{ \partial \phi }  \\
        \frac{ \partial z }{ \partial \rho } \quad \frac{ \partial z }{ \partial \phi } \quad & \frac{ \partial z }{ \partial \phi }
    \end{pmatrix}   \\
    &=
    \begin{pmatrix}
        sin \theta cos \phi \quad \rho cos \theta cos \phi \quad & - \rho sin \theta sin \phi  \\
        sin \theta sin \phi \quad \rho cos \theta sin \phi \quad & \rho sin \theta cos \phi   \\
        cos \theta \quad - \rho sin \theta \quad & 0
    \end{pmatrix}   \\
    \lvert det(J) \rvert &= r^2 sin \theta
\end{aligned}
$$

# Riemannian Geometry

Cristoffel Symbol

$$
\begin{aligned}
    \Gamma_{ij}^{k} &= \frac{\partial \vec{e^{i}}}{\partial x^{j}} \cdot \vec{e^{k}}    \\
    \frac{\partial \vec{e^{i}}}{\partial x^{j}} &= \Gamma_{ij}^{k} \vec{e^{k}}  \\
    \Gamma_{ij}^{k} &= \Gamma_{ji}^{k}  \\
    \frac{d}{d s} ( g_{jk} \xi^{j} \eta^{k} ) &= 0  \\
    \frac{\partial g_{jk}}{\partial x^{i} } &= g_{l k} \Gamma_{ji}^{l} + g_{jl} \Gamma_{ik}^{l}
\end{aligned}
$$

Covariant Derivative

$$
\begin{aligned}
    \nabla_{i} V^{j} &= \partial_{i} (e^{j} V^{j})  \\
    &= \frac{\partial V^{j}}{\partial x^{i}} e^{j} + \frac{\partial e^{j}}{\partial x^{i}} V^{j}    \\
    &= \frac{\partial V^{j}}{\partial x^{i}} e^{j} + \Gamma_{ji}^{k} e^{k} V^{j}    \\
    &= ( \frac{\partial V^{j}}{\partial x^{i}} + \Gamma_{k i}^{j} V^{k} ) e^{j}
\end{aligned}
$$

Lee Bracket

$$
\begin{aligned}
    ( \nabla_{X} Y )^{j} &= X^{i} ( \nabla_{i} Y )^{j}  \\
    &= X^{i} ( \frac{\partial Y^{j}}{\partial x^{i}} + \Gamma_{ik}^{j} Y^{k} )  \\
    \left[ X , Y \right] & \equiv \nabla_{X} Y - \nabla_{Y} X
\end{aligned}
$$

Riemann Curvature Tensor

$$
\begin{aligned}
    R( X , Y ) & \equiv [ \nabla_{X} , \nabla_{Y} ] - \nabla_{ \left[ X , Y \right] }   \\
    R_{ \sigma \mu \nu }^{\rho} & \equiv d x^{\rho} ( R( \partial_{\mu} , \partial_{\nu} ) \partial_{\sigma} )  \\
    &= \partial_{\mu} \Gamma_{\nu \sigma}^{\rho} - \partial_{\nu} \Gamma_{\mu \sigma}^{\rho} + \Gamma_{\mu \lambda}^{\rho} \Gamma_{\nu \sigma}^{\lambda} - \Gamma_{\nu \lambda}^{\rho} \Gamma_{\mu \sigma}^{\lambda}    \\
    R_{ab} & \equiv R_{acb}^{c} \\
    &= g^{cd} R_{cadb}
\end{aligned}
$$

# Field Expantion

Assume one consider Field at position \\( \vec{R} \\) with Source \\( q \\) at Position \\( \vec{r} \\), a Translational Invariant field \\( v \\) satisfies

$$
\begin{aligned}
    v( \vec{R} - \vec{r} ) &= v( \vec{r} - \vec{R} )	\\
	&= v^{0} + v^{1} + v^{2} + \cdots	\\
	&= v(\vec{R}) - \frac{1}{1!} \Sigma_{\alpha} r_{\alpha} v_{\alpha}(\vec{R}) + \frac{1}{2!} \Sigma_{\alpha\beta} r_{\alpha} r_{\beta} v_{ \alpha\beta}(\vec{R}) + \cdots   \\
    v_{ \alpha}(\vec{R}) &= \frac{ \partial v( \vec{R} - \vec{r} ) }{ \partial r_{\alpha}} \vert_{\vec{r}=0} \\
    v_{ \alpha\beta}(\vec{R}) &= \frac{ \partial^{2} v( \vec{R} - \vec{r} ) }{ \partial r_{\alpha} \partial r_{\beta} } \vert_{\vec{r}=0}
\end{aligned}
$$

# Multipole

if \\( \vec{R} \\) is far away from source, \\( v( \vec{R} - \vec{r} ) \\) satisfies the Laplace Equation and one gets

$$
\begin{aligned}
    \nabla^{2} v( \vec{R} - \vec{r} ) \vert_{\vec{r}=0} &= \Sigma_{\alpha} v_{ \alpha\alpha}(\vec{R})  \\
    &= 0    \\
    \Sigma_{\alpha\beta} r_{\alpha} r_{\beta} v_{ \alpha\beta}(\vec{R}) &= \frac{1}{d} \Sigma_{\alpha\beta} ( d r_{\alpha} r_{\beta} - \delta_{\alpha\beta} \vec{r}^2 ) v_{ \alpha\beta}(\vec{R})	\\
	&= \frac{1}{3} \Sigma_{\alpha\beta} ( 3 r_{\alpha} r_{\beta} - \delta_{\alpha\beta} \vec{r}^2 ) v_{ \alpha\beta}(\vec{R})
\end{aligned}
$$

which is the traceless Cartesian 2-Tensor

For the Coulomb case

$$
\begin{aligned}
	v( \vec{R} - \vec{r} ) & \equiv k ( ( \vec{R} - \vec{r} )^2 )^{-\frac{1}{2}}	\\
	v( \vec{R} ) &= \frac{k}{\lvert\vec{R}\rvert}	\\
	v_{\alpha}( \vec{R} ) &= - k \frac{R_{\alpha}}{\lvert\vec{R}\rvert^3}	\\
	v_{\alpha\beta}( \vec{R} ) &= k \frac{ 3 R_{\alpha} R_{\beta} - \delta_{\alpha\beta} \vec{R}^2 }{\lvert\vec{R}\rvert^5}
\end{aligned}
$$

The full Coulomb potential is

$$
\begin{aligned}
	V(\vec{R}) & \equiv k \Sigma_{i} q_{i} v( \vec{R} - \vec{r_{i}} )	\\
	&= k \frac{Q}{\lvert\vec{R}\rvert} + \frac{k}{\lvert\vec{R}\rvert^3} \Sigma_{\alpha} P_{\alpha} R_{\alpha} + \frac{k}{2\lvert\vec{R}\rvert^5} \Sigma_{\alpha\beta} Q_{\alpha\beta} R_{\alpha}R_{\beta}	\\
	Q & \equiv \Sigma_{i} q_{i}	\\
	P_{\alpha} & \equiv \Sigma_{i} q_{i} r_{i,\alpha}	\\
	Q_{\alpha\beta} & \equiv \Sigma_{i} q_{i} ( 3 r_{i,\alpha} r_{i,\beta} - \delta_{\alpha\beta} \vec{r_{i}}^2 )
\end{aligned}
$$

# Tidal Force

If there's only one Source \\( Q \\) at position \\( \vec{-R} \\) and \\( \vec{r} \\) is the field position,

$$
\begin{aligned}
	V( \vec{r} + \vec{R} ) &= V^{0} + V^{1} + V^{2} + o(r^3)	\\
	V^{0} &= k Q \frac{1}{\lvert\vec{R}\rvert}	\\
	V^{1} &= k Q \Sigma_{\alpha} r_{\alpha} \frac{-R_{\alpha}}{\lvert\vec{R}\rvert^3}	\\
	&= - k Q \frac{1}{\lvert\vec{R}\rvert^3} \vec{r} \cdot \vec{R}	\\
	V^{2} &= k Q \frac{1}{2} \Sigma_{\alpha\beta} r_{\alpha} r_{\beta}  \frac{ 3 R_{\alpha} R_{\beta} - \delta_{\alpha\beta}\vec{R}^2 }{\lvert\vec{R}\rvert^5}	\\
	&= k Q \frac{1}{2\lvert\vec{R}\rvert^5} ( 3 ( \vec{r} \cdot \vec{R} )^2 - \vec{r}^2 \vec{R}^2 )	\\
	&= k Q \frac{1}{2\lvert\vec{R}\rvert^3} ( 2 r_{\parallel}^2 - r_{\perp}^2 )
\end{aligned}
$$

Consider a Particle with Mass \\( m \\) in this potential,

$$
\begin{aligned}
	\vec{a} (\vec{r}) & = - \frac{1}{m} \nabla V( \vec{r} + \vec{R} )	\\
	&= \vec{a^{0}} + \vec{a^{1}} + o(r^2)	\\
	\vec{a^{0}} &= - \frac{1}{m} \nabla V^{1}	\\
	&= \frac{kQ}{m} \frac{\vec{R}}{\lvert\vec{R}\rvert^3}	\\
	\vec{a^{1}} &= - \frac{1}{m} \nabla V^{2}	\\
	&= \frac{kQ}{m} \frac{1}{\lvert\vec{R}\rvert^3} ( - 2 r_{\parallel} + r_{\perp} )
\end{aligned}
$$

For the Gravity case, \\( k Q = - G M m \\),

$$
\begin{aligned}
	\vec{a_{c}} &= - G M \frac{\vec{R}}{\lvert\vec{R}\rvert^3}	\\
	&= \vec{a^{0}}	\\
	\vec{a_{Tide}} & \equiv \vec{a} - \vec{a_{c}}	\\
	&= \vec{a^{1}} + o(r^2)
\end{aligned}
$$

thus, Tidal Force is repulsive in parallel direction and attractive in perpendicular direction.

# From GPT

$$Q_{ij} = \sum_{k=1}^N m_k (3r_{ik} r_{jk} - \delta_{ij} r_{kl}^2)$$

$$\mathbf{M} = -\frac{G}{2} \sum_{i,j=1}^N Q_{ij} \left( \frac{\mathbf{r}_i \times \mathbf{r}j}{r{ij}^5} \right)$$

# Problems remain
