---
title: Matrix
date: 2023-03-19
author: bosonicli
tags:
-   Ether
---

[toc]

# Diag

$$
\begin{aligned}
    if & \quad P^{\dagger}_{ n \times n } = P_{ n \times n }  \\
    esits & \quad Q_{ n \times n } \quad and \quad \Lambda_{ n \times n } \\
    where & \quad Q^{\dagger} Q = I_{n}   \\
    and & \quad \Lambda = diag_{n}(\lambda_{i})    \\
    s.t. & \quad P = Q \Lambda Q^{\dagger}  \\
    PQ &= Q \Lambda \\
    P Q_{i} &= Q_{i} \lambda_{i}
\end{aligned}
$$

# Trace

$$
\begin{aligned}
    Tr(A_{ m \times m}) & \equiv \Sigma_{i=1}^{m} A_{i,i}   \\
    Tr(( A_{ m \times n } B_{ n \times m} )_{ m \times m}) &= \Sigma_{i=1}^{m} ( A_{ m \times n } B_{ n \times m} )_{i,i}   \\
    &= \Sigma_{i=1}^{m} ( \Sigma_{j=1}^{n} A_{i,j} B_{j,i} )   \\
    &= \Sigma_{j=1}^{n} ( \Sigma_{i=1}^{m} B_{j,i} A_{i,j} )    \\
    &= Tr(( B_{ n \times m} A_{ m \times n } )_{ n \times n})
\end{aligned}
$$

# Det / Inv

$$
\begin{aligned}
    A^{-1} &= \frac{1}{det(A)} cof(A)   \\
    cof(A)_{ij} & \equiv (-)^{i+j} det(A_{ji})  \\
    \begin{pmatrix}
        a \quad b \\
        c \quad d
    \end{pmatrix}
    ^{-1} &=
    \frac{1}{ad-bc}
    \begin{pmatrix}
        d \quad & -c  \\
        -b \quad & a
    \end{pmatrix}
\end{aligned}
$$

$$
\begin{aligned}
    Tr( Q \Lambda Q^{\dagger} ) &= Tr( Q^{\dagger} Q \Lambda )  \\
    &= Tr(\Lambda)
\end{aligned}
$$

# Projection

If \\( \exist \\) hermitian matrix \\(P_{ n \times n }\\) satisfying

$$
\begin{aligned}
    P^{\dagger}_{ n \times n } &= P_{ n \times n }    \\
    P^{2}_{ n \times n } &= P_{ n \times n }
\end{aligned}
$$

Then by operating Matrix \\(P_{ n \times n }\\) on Vector \\(X_{n}\\) we got

$$
\begin{aligned}
    Y &= P X \\
    Y^{\dagger} Y &= X^{\dagger} P^{\dagger} P X    \\
    &= X^{\dagger} P P X    \\
    &= X^{\dagger} P X  \\
    &= X^{\dagger} Y    \\
    (X-Y)^{\dagger} Y &= 0  \\
    X-Y & \perp Y
\end{aligned}
$$

So \\(Y=PX\\) is a Projection of \\(X\\)

Since \\(P\\) is hermitian, it can be diagonalize

$$
\begin{aligned}
    \lambda_{i}(P) &= 0, 1  \\
    P &= Q \Lambda_{0,1} Q^{\dagger}    \\
    &=
    \begin{pmatrix}
        Q_{1} \quad Q_{2}
    \end{pmatrix}
    \begin{pmatrix}
        I_{r} \quad 0   \\
        0 \quad 0
    \end{pmatrix}
    \begin{pmatrix}
        Q_{1}^{\dagger} \\
        Q_{2}^{\dagger}
    \end{pmatrix}
    \\
    &= Q_{1} I_{r} Q_{1}^{\dagger}  \\
    &= Q_{1} (Q_{1}^{\dagger}Q_{1})^{-1} Q_{1}^{\dagger}    \\
    Tr(P) &= Tr(I_{r})   \\
    &= r(P)
\end{aligned}
$$

where \\(r=r(P)\\) is non-0 eigenvalue of \\(P\\), aka Rank of \\\(P\\)

If we consider

$$
\begin{aligned}
    P_{ n \times n } &= Q ( Q^{\dagger} Q )_{ r \times r }^{-1} Q^{\dagger} \\
    for & \quad Q_{ n \times r } \quad ( r \leq n ) \\
    P^{\dagger} &= P    \\
    P^{2} &= P  \\
    Tr(P) &= Tr( (Q^{\dagger}Q)_{ r \times r } (Q^{\dagger}Q)_{ r \times r }^{-1} ) \\
    &= Tr(I_{r})    \\
    &= r
\end{aligned}
$$

So

$$
\begin{aligned}
    P_{ n \times n } \quad is \quad rank(r) & \quad Projection \\
    & \Leftrightarrow   \\
    \exist \quad Q_{ n \times r } \quad ( r \leq n) \quad & s.t. \quad P = Q ( Q^{\dagger} Q )^{-1} Q^{\dagger}
\end{aligned}
$$
